all

code/ecdsap256/Hacl.Impl.P256.Core.fst
@@ -625,22 +625,6 @@ let scalarMultiplication #buf_type p result scalar tempBuffer =
   |CONST -> scalarMultiplicationC p result scalar tempBuffer
 
 
-val uploadBasePoint: p: point -> Stack unit 
-  (requires fun h -> live h p)
-  (ensures fun h0 _ h1 -> modifies (loc p) h0 h1 /\ 
-    as_nat h1 (gsub p (size 0) (size 4)) < prime256 /\ 
-    as_nat h1 (gsub p (size 4) (size 4)) < prime256 /\
-    as_nat h1 (gsub p (size 8) (size 4)) < prime256 /\
-      (
-	let x1 = as_nat h1 (gsub p (size 0) (size 4)) in 
-	let y1 = as_nat h1 (gsub p (size 4) (size 4)) in 
-	let z1 = as_nat h1 (gsub p (size 8) (size 4)) in 
-
-	let bpX, bpY, bpZ = basePoint in 
-
-	fromDomain_ x1  == bpX /\ fromDomain_ y1 == bpY /\ fromDomain_ z1 == bpZ
-    )
-)
 
 let uploadBasePoint p = 
     let h0 = ST.get() in 
