code/ecdsap256/Hacl.Impl.P256.ECDSA.KeyGen.fst
@@ -1,0 +1,41 @@
+module Hacl.Impl.P256.ECDSA.KeyGen
+
+
+open FStar.HyperStack.All
+open FStar.HyperStack
+module ST = FStar.HyperStack.ST
+
+open Lib.IntTypes
+open Lib.Buffer
+open Lib.ByteSequence
+
+
+val ecdsa_p256_keyGen_privateKey: random: lbuffer uint8 (size 32)
+  -> privateKey: lbuffer uint8 (size 32) -> 
+  Stack bool 
+    (requires fun h -> True)
+    (ensures fun h0 _ h1 -> True)
+
+
+let ecdsa_p256_keyGen_privateKey random result = true
+
+
+
+val ecdsa_p256_keyGen_publicKey_inner: privateKey: lbuffer uint8 (size 32) 
+  -> publibKey: lbuffer uint8 (size 64) -> 
+  Stack unit
+    (requires fun h -> True)
+    (ensures fun h0 _ h1 -> True)
+
+
+let ecdsa_p256_keyGen_publicKey_inner privateKey publicKey = ()
+
+
+val ecdsa_p256_keyGen_publicKey: privateKey: lbuffer uint8 (size 32) 
+  -> publicKey: lbuffer uint8 (size 64) ->
+  Stack bool
+    (requires fun h -> True)
+    (ensures fun h0 _ h1 -> True)
+
+
+let ecdsa_p256_keyGen_publicKey privateKey publicKey = true
