code/ecdsap256/Hacl.Impl.Q.Test.fst
@@ -1,0 +1,33 @@
+module Hacl.Impl.Q.Test
+
+open Spec.P256
+open Spec.P256.Definitions
+open Spec.P256.Lemmas
+open Spec.P256.MontgomeryMultiplication
+open FStar.Mul
+
+open FStar.Calc
+open FStar.Tactics
+
+#set-options "--z3rlimit 200 --fuel 0 --ifuel 0" 
+
+val lemmaBPBlinding: x0: nat -> y0: nat -> z0: nat -> r: nat 
+  -> x1: nat 
+  -> y1: nat  -> z1: nat -> 
+  Lemma 
+   (
+    let resultFromDomain = fromDomain_ x1, fromDomain_ y1, fromDomain_ z1 in 
+    let rnX, rnY, rnZ = _norm resultFromDomain in 
+    rnX == x0)
+
+
+let lemmaBPBlinding x0 y0 z0 r x1 y1 z1 =
+  assert((fromDomain_ z0 * r % prime256) >= 0);
+  admit();
+  calc(==)
+  {
+   5;
+    (==) {}
+     5;
+  };
+  admit()
